<?xml version="1.0"?>


<!DOCTYPE rdf:RDF [
    <!ENTITY owl "http://www.w3.org/2002/07/owl#" >
    <!ENTITY obo "http://purl.obolibrary.org/obo/" >
    <!ENTITY xsd "http://www.w3.org/2001/XMLSchema#" >
    <!ENTITY snap "http://www.ifomis.org/bfo/1.1/snap#" >
    <!ENTITY rdfs "http://www.w3.org/2000/01/rdf-schema#" >
    <!ENTITY rdf "http://www.w3.org/1999/02/22-rdf-syntax-ns#" >
]>


<rdf:RDF xmlns="&obo;example/"
     xml:base="&obo;example/"
     xmlns:obo="http://purl.obolibrary.org/obo/"
     xmlns:rdfs="http://www.w3.org/2000/01/rdf-schema#"
     xmlns:snap="http://www.ifomis.org/bfo/1.1/snap#"
     xmlns:owl="http://www.w3.org/2002/07/owl#"
     xmlns:xsd="http://www.w3.org/2001/XMLSchema#"
     xmlns:rdf="http://www.w3.org/1999/02/22-rdf-syntax-ns#">
    <owl:Ontology rdf:about="&obo;example/bfo-rel.owl">
        <owl:imports rdf:resource="&obo;example/bfo-classes.owl"/>
    </owl:Ontology>
    


    <!-- 
    ///////////////////////////////////////////////////////////////////////////////////////
    //
    // Annotation properties
    //
    ///////////////////////////////////////////////////////////////////////////////////////
     -->

    <owl:AnnotationProperty rdf:about="&rdfs;label"/>
    


    <!-- 
    ///////////////////////////////////////////////////////////////////////////////////////
    //
    // Datatypes
    //
    ///////////////////////////////////////////////////////////////////////////////////////
     -->

    


    <!-- 
    ///////////////////////////////////////////////////////////////////////////////////////
    //
    // Object Properties
    //
    ///////////////////////////////////////////////////////////////////////////////////////
     -->

    
    <owl:ObjectProperty rdf:about="&obo;example/part_of_process">
        <owl:propertyChainAxiom rdf:parseType="Collection">
            <rdf:Description rdf:about="&obo;example/general_part_of"/>
            <rdf:Description rdf:about="&obo;example/self_o"/>
        </owl:propertyChainAxiom>
    </owl:ObjectProperty>

    <!-- http://purl.obolibrary.org/obo/example/process_has_part -->

    <owl:ObjectProperty rdf:about="&obo;example/process_has_part">
        <owl:propertyChainAxiom rdf:parseType="Collection">
            <rdf:Description rdf:about="&obo;example/general_has_part"/>
            <rdf:Description rdf:about="&obo;example/self_o"/>
        </owl:propertyChainAxiom>
    </owl:ObjectProperty>




    <!-- http://purl.obolibrary.org/obo/example/has_part_at_all_times -->

    <owl:ObjectProperty rdf:about="&obo;example/has_part_at_all_times">
        <rdf:type rdf:resource="&owl;TransitiveProperty"/>
        <rdfs:label xml:lang="en">has part at all times</rdfs:label>
        <obo:IAO_0000115 xml:lang="en">For all times in temporal projection of the subject&#39;s course the subject is part of the object. This implies the object exists at all times that the subject exists.</obo:IAO_0000115>
        <rdfs:range rdf:resource="&obo;example/c"/>
        <rdfs:domain rdf:resource="&obo;example/c"/>
        <rdfs:subPropertyOf rdf:resource="&obo;example/has_part_at_some_time"/>
    </owl:ObjectProperty>
    


    <!-- http://purl.obolibrary.org/obo/example/has_part_at_some_time -->

    <owl:ObjectProperty rdf:about="&obo;example/has_part_at_some_time">
        <rdfs:label xml:lang="en">has part at some time</rdfs:label>
        <obo:IAO_0000116 xml:lang="en">The relation is not transitive, as if a has part b at some t1 and b has part c and some time t2, the relation would only be transitive when t1 = t2, which isn&#39;t part of the definition.</obo:IAO_0000116>
        <obo:IAO_0000115 xml:lang="en">There exists some time instant in the temporal projection of the subject&#39;s course at which time the subject is part of the object. This implies the object exists at that time. </obo:IAO_0000115>
        <rdfs:range rdf:resource="&obo;example/c"/>
        <rdfs:domain rdf:resource="&obo;example/c"/>
        <owl:inverseOf rdf:resource="&obo;example/part_of_at_some_time"/>
        <owl:propertyChainAxiom rdf:parseType="Collection">
            <rdf:Description rdf:about="&obo;example/has_part_during"/>
            <rdf:Description rdf:about="&obo;example/life_of"/>
        </owl:propertyChainAxiom>
    </owl:ObjectProperty>
    


    <!-- http://purl.obolibrary.org/obo/example/has_part_during -->

    <owl:ObjectProperty rdf:about="&obo;example/has_part_during">
        <rdfs:label xml:lang="en">has part during</rdfs:label>
        <obo:IAO_0000115 xml:lang="en">a continuant c has part during some process p iff p is a temporal part of a course and for all times t in the temporal projection of the course c has part (course-of course) a t</obo:IAO_0000115>
        <obo:IAO_0000116 xml:lang="en">the constraint on temporal part of is that the part and the whole occupy the same spatial region at all times in the temporal projection of the whole. But the whole may extend longer, temporally</obo:IAO_0000116>
        <rdfs:domain rdf:resource="&obo;example/c"/>
        <owl:propertyChainAxiom rdf:parseType="Collection">
            <rdf:Description rdf:about="&obo;example/has_part_during"/>
            <rdf:Description rdf:about="&obo;example/part_of_process"/>
        </owl:propertyChainAxiom>
        <rdfs:range>
            <owl:Restriction>
                <owl:onProperty rdf:resource="&obo;example/temporal_part_of"/>
                <owl:someValuesFrom rdf:resource="&obo;example/course"/>
            </owl:Restriction>
        </rdfs:range>
    </owl:ObjectProperty>
    


    <!-- http://purl.obolibrary.org/obo/example/has_participant -->

    <owl:ObjectProperty rdf:about="&obo;example/has_participant">
        <rdfs:label xml:lang="en">has_participant at some time</rdfs:label>
        <obo:IAO_0000115 xml:lang="en">A relation between an ocurrent and a continuant where there exists some time in the temporal projection of the occurrent at which the subject participates in the object.</obo:IAO_0000115>
        <obo:IAO_0000116 xml:lang="en">This corresponds to the quanitification over time as was stated for the class relation definition in Relations in Biomedical Ontology

A suitable target for participates_in relations in the OBO to OWL conversion</obo:IAO_0000116>
        <rdfs:range rdf:resource="&obo;example/c"/>
        <rdfs:domain rdf:resource="&obo;example/o"/>
    </owl:ObjectProperty>
    


    <!-- http://purl.obolibrary.org/obo/example/has_proper_part_at_all_times -->

    <owl:ObjectProperty rdf:about="&obo;example/has_proper_part_at_all_times">
        <rdfs:label xml:lang="en">has proper part at all times</rdfs:label>
        <obo:IAO_0000115 xml:lang="en">For all  times t in temporal projection of the subject&#39;s course the subject has a proper part the object at t</obo:IAO_0000115>
        <obo:IAO_0000116 xml:lang="en">This relation will probably be removed - we can&#39;t define it as transitive as transitivity and disjoint properties together violate the OWL general constraints.
</obo:IAO_0000116>
        <rdfs:range rdf:resource="&obo;example/c"/>
        <rdfs:domain rdf:resource="&obo;example/c"/>
        <rdfs:subPropertyOf rdf:resource="&obo;example/has_part_at_all_times"/>
        <owl:propertyDisjointWith rdf:resource="&obo;example/self_c"/>
    </owl:ObjectProperty>
    


    <!-- http://purl.obolibrary.org/obo/example/has_proper_part_at_some_time -->

    <owl:ObjectProperty rdf:about="&obo;example/has_proper_part_at_some_time">
        <rdfs:label xml:lang="en">has proper part at some time</rdfs:label>
        <obo:IAO_0000115 xml:lang="en">For some time in temporal projection of the subject&#39;s course the subject has a proper part the object . </obo:IAO_0000115>
        <rdfs:subPropertyOf rdf:resource="&obo;example/has_part_at_some_time"/>
        <owl:propertyDisjointWith rdf:resource="&obo;example/self_c"/>
    </owl:ObjectProperty>
    


    <!-- http://purl.obolibrary.org/obo/example/part_of_at_all_times -->

    <owl:ObjectProperty rdf:about="&obo;example/part_of_at_all_times">
        <rdf:type rdf:resource="&owl;TransitiveProperty"/>
        <rdfs:label>part of at all times</rdfs:label>
        <obo:IAO_0000115 xml:lang="en">For all times in temporal projection of the subject&#39;s course the subject has part the object. This implies the object exists at all times that the subject exists.</obo:IAO_0000115>
        <rdfs:range rdf:resource="&obo;example/c"/>
        <rdfs:domain rdf:resource="&obo;example/c"/>
        <rdfs:subPropertyOf rdf:resource="&obo;example/part_of_at_some_time"/>
        <owl:propertyChainAxiom rdf:parseType="Collection">
            <rdf:Description rdf:about="&obo;example/general_part_of"/>
            <rdf:Description rdf:about="&obo;example/self_c"/>
        </owl:propertyChainAxiom>
    </owl:ObjectProperty>
    


    <!-- http://purl.obolibrary.org/obo/example/part_of_at_some_time -->

    <owl:ObjectProperty rdf:about="&obo;example/part_of_at_some_time">
        <rdfs:label>part of at some time</rdfs:label>
        <obo:IAO_0000115 xml:lang="en">There exists some time instant in the temporal projection of the subject&#39;s course at which time the subject has part the object. This implies the object exists at that time. </obo:IAO_0000115>
        <rdfs:domain rdf:resource="&obo;example/c"/>
        <rdfs:range rdf:resource="&obo;example/c"/>
        <owl:propertyChainAxiom rdf:parseType="Collection">
            <rdf:Description rdf:about="&obo;example/part_of_during"/>
            <rdf:Description rdf:about="&obo;example/life_of"/>
        </owl:propertyChainAxiom>
    </owl:ObjectProperty>
    


    <!-- http://purl.obolibrary.org/obo/example/part_of_during -->

    <owl:ObjectProperty rdf:about="&obo;example/part_of_during">
        <rdfs:label>part of during</rdfs:label>
        <obo:IAO_0000115 xml:lang="en">a continuant c is part of during some process p iff p is a temporal part of a course and for all times t in the temporal projection of the course c part of (course-of course) a t</obo:IAO_0000115>
        <obo:IAO_0000116 xml:lang="en">the constraint on temporal part of is that the part and the whole occupy the same spatial region at all times in the temporal projection of the whole. But the whole may extend longer, temporally</obo:IAO_0000116>
        <rdfs:domain rdf:resource="&obo;example/c"/>
        <owl:propertyChainAxiom rdf:parseType="Collection">
            <rdf:Description rdf:about="&obo;example/part_of_during"/>
            <rdf:Description rdf:about="&obo;example/part_of_process"/>
        </owl:propertyChainAxiom>
        <rdfs:range>
            <owl:Restriction>
                <owl:onProperty rdf:resource="&obo;example/temporal_part_of"/>
                <owl:someValuesFrom rdf:resource="&obo;example/course"/>
            </owl:Restriction>
        </rdfs:range>
    </owl:ObjectProperty>
    

    <!-- http://purl.obolibrary.org/obo/example/participates_in -->

    <owl:ObjectProperty rdf:about="&obo;example/participates_in">
        <rdfs:label xml:lang="en">participates_in at some time</rdfs:label>
        <obo:IAO_0000115 xml:lang="en">A relation between a continuant and an occurrent where there exists some time in the temporal projection of the subject&#39;s course at which the subject participates in the object. </obo:IAO_0000115>
        <obo:IAO_0000116 xml:lang="en">This corresponds to the quanitification over time as was stated for the class relation definition in Relations in Biomedical Ontology

A suitable target for participates_in relations in the OBO to OWL conversion</obo:IAO_0000116>
        <owl:inverseOf rdf:resource="&obo;example/has_participant"/>
    </owl:ObjectProperty>
    



    <!-- http://purl.obolibrary.org/obo/example/proper_part_of_at_some_time -->

    <owl:ObjectProperty rdf:about="&obo;example/proper_part_of_at_some_time">
        <rdfs:label xml:lang="en">proper part of at some time</rdfs:label>
        <obo:IAO_0000115 xml:lang="en">For some time in temporal projection of the subject&#39;s course the subject is a proper part the object . </obo:IAO_0000115>
        <rdfs:subPropertyOf rdf:resource="&obo;example/part_of_at_some_time"/>
        <owl:propertyDisjointWith rdf:resource="&obo;example/self_c"/>
    </owl:ObjectProperty>
    


    <!-- http://purl.obolibrary.org/obo/example/self_c -->

    <owl:ObjectProperty rdf:about="&obo;example/self_c">
        <rdfs:label xml:lang="en">self c</rdfs:label>
        <obo:IAO_0000115 xml:lang="en">A relation that holds for any continuant instance, relating the occurrent to itself. Identity.</obo:IAO_0000115>
        <obo:IAO_0000116>Here only to support reasoning. It allows us define part of relations as locally reflexive, as well as proper parthood by excluding these self relations. Effectively identity, restricted to occurrents. If we defined part of relations to be globally reflexive, then we would have it applied to every entity, including those for which part_of might not make sense. As an example, it is not clear whether it makes sense to say realizable entities have parts.</obo:IAO_0000116>
        <rdfs:range rdf:resource="&obo;example/c"/>
        <rdfs:domain rdf:resource="&obo;example/c"/>
        <rdfs:subPropertyOf rdf:resource="&obo;example/general_has_part"/>
        <rdfs:subPropertyOf rdf:resource="&obo;example/general_part_of"/>
        <rdfs:subPropertyOf rdf:resource="&obo;example/has_part_at_all_times"/>
        <rdfs:subPropertyOf rdf:resource="&obo;example/part_of_at_all_times"/>
    </owl:ObjectProperty>
    


    <!-- http://purl.obolibrary.org/obo/example/self_o -->

    <owl:ObjectProperty rdf:about="&obo;example/self_o">
        <rdfs:label xml:lang="en">self o</rdfs:label>
        <obo:IAO_0000115 xml:lang="en">A relation that holds for any occurrent instance, relating the occurrent to itself. </obo:IAO_0000115>
        <obo:IAO_0000116 xml:lang="en">Here only to support reasoning. It allows us define part of relations as locally reflexive, as well as proper parthood by excluding these self relations. Effectively identity, restricted to occurrents. If we defined part of relations to be globally reflexive, then we would have it applied to every entity, including those for which part_of might not make sense. As an example, it is not clear whether it makes sense to say realizable entities have parts.</obo:IAO_0000116>
        <rdfs:subPropertyOf rdf:resource="&obo;example/general_has_part"/>
        <rdfs:subPropertyOf rdf:resource="&obo;example/general_part_of"/>
        <rdfs:domain rdf:resource="&obo;example/o"/>
        <rdfs:range rdf:resource="&obo;example/o"/>
        <rdfs:subPropertyOf rdf:resource="&obo;example/part_of_process"/>
        <rdfs:subPropertyOf rdf:resource="&obo;example/temporal_part_of"/>
    </owl:ObjectProperty>
    

    <!-- http://www.w3.org/2002/07/owl#topObjectProperty -->

    <owl:ObjectProperty rdf:about="&owl;topObjectProperty"/>
    


    <!-- 
    ///////////////////////////////////////////////////////////////////////////////////////
    //
    // Classes
    //
    ///////////////////////////////////////////////////////////////////////////////////////
     -->

    



    <!-- 
    ///////////////////////////////////////////////////////////////////////////////////////
    //
    // Individuals
    //
    ///////////////////////////////////////////////////////////////////////////////////////
     -->

</rdf:RDF>



<!-- Generated by the OWL API (version 3.2.3.22702) http://owlapi.sourceforge.net -->

